\documentclass{article}

\usepackage{amsmath}
\usepackage{amssymb}
\usepackage{graphicx}

\begin{document}


Ivan Lin\newline{}
Dr. Esther Arkin\newline{}
AMS301\newline{}
4/18/17

\begin{center}
  Homework 9b
\end{center}

\underline{Section 6.2 Problem 8}

Find the coefficient of $x^{24}$ in $(x+x^2+x^3+x^4+x^5)^8$\newline{}

$g(x)=(x+x^2+x^3+x^4+x^5)^8$\newline{}
$g(x)=[x(1+x+x^2+x^3+x^4)]^8$\newline{}
$g(x)=x^8(1+x+x^2+x^3+x^4)^8$\newline{}
let $f(x)=(1+x+x^2+x^3+x^4)^8$\newline{}
coefficient of $x^{24}$ in $g(x)$ is equal to coefficient of $x^{24-8}=x^{16}$ in $f(x)$\newline{}
$f(x)=(1+x+x^2+x^3+x^4)^8$\newline{}
$f(x)=\frac{1-x^{4}}{1-x}^8$\newline{}
$f(x)=(1-x^4)^8\frac{1}{1-x}^8$\newline{}
$a=(1-x^4)^8=1-\dbinom{8}{1}x^4+\dbinom{8}{2}x^8+...+\dbinom{8}{8}x^{32}$\newline{}
$b=\frac{1}{1-x}^8=1+\dbinom{8}{1}x+\dbinom{9}{2}x^2+...+\dbinom{23}{16}x^{16}+...$\newline{}
coefficient of $x^{16}$ is $a_0b_{16}+a_1b_{15}+...+a_{16}b_0$\newline{}
$1\dbinom{23}{16}+\dbinom{8}{1}\dbinom{18}{12}+\dbinom{8}{2}\dbinom{15}{8}+\dbinom{8}{3}\dbinom{11}{4}+\dbinom{8}{4}*1$\newline{}

\underline{Section 6.2 Problem 14}

Find the coefficient of $x^{18}$ in $(1+x^3+x^6+...)^6$\newline{}

$g(x)=(1+x^3+x^6+...)^6$\newline{}
let $z=x^3$\newline{}
$g(x)=(1+z+z^2+...)^6$\newline{}
$g(x)=\frac{1}{1-z}^6$\newline{}
$g(x)=\frac{1}{(1-z)^6}$\newline{}
$g(x)=1+\dbinom{6}{1}z+\dbinom{7}{2}z^2+...+\dbinom{11}{6}z^6+...$\newline{}
coefficient of $x^{18}$ is coefficient of $z^6$\newline{}
$\dbinom{11}{6}$\newline{}

\underline{Section 6.2 Problem 22}

How many ways are there to get a sum of 25 when 10 distinct dice are rolled?\newline{}

This question can be modelled as $e_1+e_2+...+e_{10}=25$ or alternatively the coefficient of $x^{25}$ in $(1+x^1+x^2+...+x^6)^{10}$\newline{}

$g(x)=(x^1+x^2+...+x^6)^{10}$\newline{}
$g(x)=[x(1+x^1+x^2+...+x^5)]^{10}$\newline{}
$g(x)=x^{10}\frac{1-x^{6}}{1-x}^{10}$\newline{}
coefficient of $x^{25}$ is coefficient of $x^{15}$ in $\frac{1-x^{6}}{1-x}^{10}$\newline{}
$g(x)=(1-x^{6})^{10}\frac{1}{1-x}^{10}$\newline{}
$a=(1-x^{6})^{10}=1-\dbinom{10}{1}x^6+\dbinom{10}{2}x^{12}-...+\dbinom{10}{10}x^{60}$\newline{}
$b=\frac{1}{1-x}^{10}=1+\dbinom{10}{1}x+\dbinom{11}{2}x^2+...+\dbinom{24}{15}x^{15}+...$\newline{}
coefficient of $x^{15}$\newline{}
$1\dbinom{24}{15}+\dbinom{10}{1}\dbinom{18}{9}+\dbinom{10}{2}\dbinom{12}{3}$\newline{} 

\end{document}
