\documentclass{article}

\usepackage[english]{babel}
\usepackage[utf8x]{inputenc}
\usepackage{amsmath}
\begin{document}

Ivan Lin

Dr. Michael Bender

CSE150 - Honors Foundations of Computer Science Fall 2016

\begin{center}
Homework 1a
\end{center}
\underline{Problem 1}
Write $P\implies Q$ using $\lor$ and $\sim$. Show that your two representations are equivalent.
\begin{center}
$(P\implies Q)\iff (\sim P \lor Q)$

\begin{tabular}{|l|l|l|l|l|}
  \hline $P$ & $Q$ & $\sim P$ & $P\implies Q$ & $\sim P \lor Q$\\  
  \hline T & T & F & T & T\\
  \hline T & F & F & F & F\\
  \hline F & T & T & T & T\\
  \hline F & F & T & T & T\\
  \hline
\end{tabular}
\end{center}

\underline{Problem 2}
Prove that the propositional formulas
\begin{center}
  $P\lor Q\lor R$
\end{center}
and
\begin{center}
  $(P\land\sim Q)\lor(Q\land\sim R)\lor(R\land\sim P)\lor(P\land Q\land R)$
\end{center}
are equivalent.

\begin{center}
\begin{tabular}{|l|l|l|l|l|l|l|l|l|l|}
  \hline $P$ & $Q$ & $R$ & $\sim P$ & $\sim Q$ & $\sim R$ & $P\land \sim Q$ & $Q\land \sim R$ & $R\land \sim P$ & $P\lor Q\lor R$\\
  \hline T & T & T & F & F & F & F & F & F & T \\ 
  \hline T & T & F & F & F & T & F & T & F & F \\
  \hline T & F & T & F & T & F & T & F & F & F \\
  \hline F & T & T & T & F & F & F & F & T & F \\
  \hline T & F & F & F & T & T & T & F & F & F \\
  \hline F & F & T & T & T & F & F & F & T & F \\
  \hline F & T & F & T & F & T & F & T & F & F \\
  \hline F & F & F & T & T & T & F & F & F & F \\
  \hline
\end{tabular}
\begin{tabular}{|l|l|}
  \hline $(P\land\sim Q)\lor(Q\land\sim R)\lor(R\land\sim P)\lor(P\land Q\land R)$ & $P\lor Q\lor R$\\
  \hline T & T\\
  \hline T & T\\
  \hline T & T\\
  \hline T & T\\
  \hline T & T\\
  \hline T & T\\
  \hline T & T\\
  \hline F & F\\
  \hline
\end{tabular}
\end{center}


\underline{Problem 3}
(a) Write the biconditional ($\Leftrightarrow$) using only implies ($\implies$) and and ($\land$). Prove that the new version is equivalent.
\begin{center}
$(P\Leftrightarrow Q)\iff (P\implies Q)\land (Q\implies P)$

  \begin{tabular}{|l|l|l|l|l|l|}
    \hline $P$&$Q$&$P\implies Q$&$Q\implies P$&$P(\implies Q)\land (Q\implies P)$&$P\Leftrightarrow Q$\\
    \hline T&T&T&T&T&T \\
    \hline T&F&F&F&F&F \\
    \hline F&T&T&T&F&F \\
    \hline F&F&T&T&T&T \\
    \hline
  \end{tabular}
\end{center}
(b) Write it using only $\lor$ and $\sim$. Show your derivation.
\begin{center}
  $(P\Leftrightarrow Q)\iff (P\implies Q)\land (Q\implies P)$

  given  $A\iff \sim (P\implies Q), B\iff \sim (Q\implies P)$

  $(P\implies Q)\land (Q\implies P)\iff (\sim A\land \sim B)$

  $(\sim A\land \sim B) \iff \sim(A\lor B)$ by De Morgan's Laws

  $\sim(A\lor B)\iff \sim(\sim (P\implies Q) \lor \sim (Q\implies P))$
  
  since $(P\implies Q)\iff(\sim P \lor Q)$

  $\sim(\sim (P\implies Q) \lor \sim (Q\implies P)) \iff \sim(\sim (\sim P \lor Q) \lor \sim (\sim Q\lor P))$
\end{center}
\end{document}
